---
aliases: 
tags: 
- public
- knowledge
title: Differenzialrechnung
date created: "2023-03-14T04:01:04"
date modified: "2023-03-14T05:19:39"
---

# Differenzialrechnung

## Differentiationsregeln

[[Potenzfunktion]]
$$f(x) = x^n \implies f'(x) = n \cdot x^{n-1}$$
[[Konstante Funktion]]
$$ f(x) = c \implies f'(x) = 0 $$
[[Eulerische Funktion]]
$$ f(x) = e^x \implies f'(x) = e^x $$
[[Exponentialfunktion]]
$$ f(x) = a^x \implies f'(x) = ln(a) \cdot a^x $$
[[Logarithmusfunktion]]
$$ f(x) = ln(x) \implies f'(x) = \frac{1}{x}$$
Faktorregel
$$ f(x) = a \cdot g(x) \implies f'(x) = (a \cdot g'(x))' = a \cdot g'(x) $$
$$ f(x) = a \cdot x^n \implies f'(x) = a \cdot n \cdot x^{n-1}$$
Summenregel
$$ (f(x) + g(x))' = f'(x) + g'(x) $$
Produkteregel
$$ (f(x) \cdot g(x))' = f'(x) \cdot g(x) + f(x) \cdot g'(x)$$
Quotientenregel
$$ (\frac{f(x)}{g(x)})' = \frac{f'(x) \cdot g(x) - f(x) \cdot g'(x)}{(g(x))^2}$$
$$ (\frac{1}{g(x)})' = \frac{-g'(x)}{(g(x))^2} $$
Kettenregel
$$ f(g(x)) \implies (f(g(x)))' = f'(g(x)) \cdot g'(x) $$
